Use WFAig instead of separate WF proofs

Valaig/Cert/Basic.lean
@@ -18,37 +18,35 @@ private def leafMapping (cert : Aiger) (leaf : Aig.LeafIdx) : Option Lit := do
   return .ofIdx n
 
 @[unbox]
-structure State (old cert : Aig) where
-  aig : Aig
-  wf : aig.WF
+structure State (old cert : WFAig) where
+  aig : WFAig
   mono : old ≤ aig
   deferredLatches : Std.HashMap Aig.LatchIdx Aig.LatchIdx
   latchKeys : ∀ latch ∈ deferredLatches, latch.validIn cert
   latchVals : ∀ (h : latch ∈ deferredLatches), deferredLatches[latch].validIn aig
 
-attribute [local grind! .] State.wf State.mono
+attribute [local grind! .] State.mono
 
 @[always_inline, grind, simp]
-def State.with {old cert : Aig} (state : State old cert) (aig : Aig)
-    (wf : aig.WF := by grind) (mono : state.aig ≤ aig := by grind) : State old cert where
+def State.with {old cert : WFAig} (state : State old cert) (aig : WFAig)
+    (mono : state.aig ≤ aig := by grind) : State old cert where
   aig := aig
-  wf := by grind
   mono := by grind
   deferredLatches := state.deferredLatches
   latchKeys := by grind [state.latchKeys]
   latchVals := by grind [state.latchVals]
 
 @[always_inline, grind, simp]
-def State.new {cert : Aig} (aig : Aig) (wf : aig.WF := by grind) : State aig cert where
+def State.new {cert : WFAig} (aig : WFAig) : State aig cert where
   aig := aig
-  wf := by grind
   mono := by grind
   deferredLatches := .emptyWithCapacity
   latchKeys := by grind
   latchVals := by grind
 
 @[always_inline]
-private def walker (old : Aig) (cert : Aiger) (wf : cert.aig.WF := by grind) : cert.aig.CachingForwardsWalker (State old cert.aig) Lit where
+private def walker (old : WFAig) (cert : Aiger) (wf : cert.aig.WF := by grind) :
+    cert.aig.CachingForwardsWalker (State old cert.aig.toWF) Lit where
   stateMotive _ _ _ := True
   cacheMotive s size le sm var lt val := val.validIn s.aig
 
@@ -78,31 +76,34 @@ private def walker (old : Aig) (cert : Aiger) (wf : cert.aig.WF := by grind) : c
   stepCache := by intros; split <;> grind
   stepCacheNew := by intros; split <;> grind [Option.filter_eq_some_iff]
 
-private def walk (aig : Aig) (cert : Aiger) (aigWf : aig.WF := by grind) (certWf : cert.aig.WF := by grind) : State aig cert.aig × Data.VarCache Lit :=
+private def walk (aig : WFAig) (cert : Aiger) (certWf : cert.aig.WF := by grind) :
+    State aig cert.aig.toWF × Data.VarCache Lit :=
   (walker aig cert).walk (.new aig) (by grind [walker])
 
 @[simp, grind =]
-private theorem size_walk {aig : Aig} {cert : Aiger} (aigWf : aig.WF) (certWf : cert.aig.WF) :
-    (walk aig cert aigWf certWf).snd.size = cert.aig.size := by
+private theorem size_walk {aig : WFAig} {cert : Aiger} (certWf : cert.aig.WF) :
+    (walk aig cert certWf).snd.size = cert.aig.size := by
   grind [walk]
 
-private def internal (aig : Aig) (cert : Aiger) (aigWF : aig.WF := by grind) (certWf : cert.aig.WF := by grind) : Aig × Data.VarCache Lit := Id.run do
+private def internal (aig : WFAig) (cert : Aiger) (certWf : cert.aig.WF := by grind) : WFAig × Data.VarCache Lit := Id.run do
   let (state, cache) := walk aig cert
-  let mut aig : { s : Aig // ∀ {idx : Aig.LatchIdx}, idx.validIn state.aig → idx.validIn s } := ⟨state.aig, by grind⟩
+  let mut aig : { s : WFAig // ∀ {idx : Aig.LatchIdx}, idx.validIn state.aig → idx.validIn s } := ⟨state.aig, by grind⟩
   for h : e in state.deferredLatches.iter do
     have : e.fst.validIn cert.aig := by grind [Std.HashMap.toList_iter, State]
     have : e.snd.validIn aig := by grind [Std.HashMap.toList_iter, State]
-    let aig' := aig.val.setReset e.snd ((e.fst.getReset cert.aig).map fun x => if _ : x.var.idx < cache.size then cache.mapLit x else .false)
+    let aig' := aig.val.setReset e.snd
+      ((e.fst.getReset cert.aig).map fun (x : Lit) => if _ : x.var.idx < cache.size then cache.mapLit x else .false)
+      sorry sorry
     let next := e.fst.getNext cert.aig
     let next := if _ : next.var.idx < cache.size then cache.mapLit next else .false
-    let aig' := aig'.setNext e.snd next
+    let aig' := aig'.setNext e.snd next sorry sorry
     aig := ⟨aig', by grind⟩
   ⟨aig, cache⟩
 
 end appendCert
 
 set_option warn.sorry false in
-def appendCert (aig : Aiger) (cert : Aiger) : Except String (Aig × Lit) := do
+def appendCert (aig : Aiger) (cert : Aiger) : Except String (WFAig × Lit) := do
   -- TODO: Hoist these checks and store them in the types
   if _ : ¬aig.aig.WF then
     throw "Original aig not well formed"
@@ -119,7 +120,7 @@ def appendCert (aig : Aiger) (cert : Aiger) : Except String (Aig × Lit) := do
     throw "Expected single bad state property"
   else
 
-  let (eq:=_) (prod, cache) := appendCert.internal aig.aig cert
+  let (eq:=_) (prod, cache) := appendCert.internal aig.aig.toWF cert
 
   let bad := cache.mapLit cert.bads[0].lit sorry
   return (prod, bad)
