Valaig/Tools/ValaigCert.lean
@@ -19,7 +19,7 @@ def liftCoreM (action : Lean.CoreM α) : IO α := do
   let state := { env := env }
   action.toIO' ctx state
 
-def checkUnsat (aig : Aig) (lit : Lit) (reset : Bool) (valid : lit.validIn aig := by grind) (wf : aig.WF := by grind) : IO (Except String Unit) := do
+def checkUnsat (aig : WFAig) (lit : Lit) (reset : Bool) (valid : lit.validIn aig := by grind) : IO (Except String Unit) := do
   let res := Sat.toStd aig reset
   IO.print s!"({res.fst.decls.size} nodes) "
   let entry : Std.Sat.AIG.Entrypoint Aig.LeafIdx := .mk res.fst (res.snd ⟨lit, valid⟩)
@@ -32,14 +32,14 @@ def run (model cert : String) : IO Unit := do
   IO.println "Reading model"
   let model ← IO.FS.Handle.mk model .read
   let (_, model) ← IO.ofExcept <| Valaig.Aiger.parse <| ← model.readBinToEnd
-
+  
   let bad := model.bads[0]!.lit
 
   IO.println "Reading certificate"
   let cert ← IO.FS.Handle.mk cert .read
   let (_, cert) ← IO.ofExcept <| Valaig.Aiger.parse <| ← cert.readBinToEnd
 
-  let modelaig := Transform.twoLevelSimp model.aig sorry
+  let modelaig := Transform.twoLevelSimp (model.aig.toWF sorry)
   let model := { model with aig := modelaig }
 
   IO.println "Constructing product circuit"
@@ -49,20 +49,20 @@ def run (model cert : String) : IO Unit := do
 
   -- Check that in a reset state the invariant holds
   IO.print "Init: "
-  IO.ofExcept <| ← checkUnsat product invbad true sorry sorry
+  IO.ofExcept <| ← checkUnsat product invbad true sorry
   IO.println "ok"
 
   -- Check that whenever the invariant holds, the original property does too
-  let (product, imp) := product.addAndRaw invbad.invert bad
+  let (product, imp) := product.addAndRaw invbad.invert bad sorry sorry
   IO.print "Implication: "
-  IO.ofExcept <| ← checkUnsat product imp false sorry sorry
+  IO.ofExcept <| ← checkUnsat product imp false sorry
   IO.println "ok"
 
   -- Check that the invariant is inductive
-  let (product, map) := Transform.unroll product sorry
-  let (product, imp) := product.addAndRaw invbad.invert (map.mapLit invbad sorry)
+  let (product, map) := Transform.unroll product
+  let (product, imp) := product.addAndRaw invbad.invert (map.mapLit invbad sorry) sorry sorry
   IO.print "Consecution: "
-  IO.ofExcept <| ← checkUnsat product imp false sorry sorry
+  IO.ofExcept <| ← checkUnsat product imp false sorry
   IO.println "ok"
 
   return ()
