Valaig/Transform/Unroll.lean
@@ -9,8 +9,8 @@ open Aig
 namespace unroll
 
 @[always_inline]
-private def walker (old : Aig) : old.CachingForwardsWalker Aig Lit where
-  stateMotive aig size le := aig.WF ∧ old ≤ aig
+private def walker (old : WFAig) : old.CachingForwardsWalker WFAig Lit where
+  stateMotive aig size le := old ≤ aig
   cacheMotive aig size le sm var lt lit := lit.validIn aig
 
   step var aig cache valid size sm cm :=
@@ -18,7 +18,7 @@ private def walker (old : Aig) : old.CachingForwardsWalker Aig Lit where
     | .false       => (aig, .false)
     | .and lhs rhs => let (eq:=_) (aig, var) := aig.addAnd (cache.mapLit lhs) (cache.mapLit rhs)
                       (aig, var)
-    | .input _     => let (eq:=_) (aig, idx) := aig.addInput; (aig, idx.getVar aig)
+    | .input _     => let (eq:=h) (aig, idx) := aig.addInput; (aig, idx.getVar aig)
     | .latch idx   => (aig, idx.getNext aig)
 
   stepState := by intros; split <;> grind
@@ -33,7 +33,7 @@ end unroll
 
   TODO: Strashing whilst unrolling
 -/
-def unroll (aig : Aig) (wf : aig.WF := by grind) : Aig × Data.VarCache Lit :=
+def unroll (aig : WFAig) : WFAig × Data.VarCache Lit :=
   (unroll.walker aig).walk aig (by grind [unroll.walker])
 
 end Valaig.Transform
